fixed huffman tree

examples/deflate/deflateScript.sml
@@ -59,25 +59,85 @@ End
 
 EVAL “next_code (bl_count [3;3;3;3;3;2;4;4])”;
 
+(* binary numbers in little-endian format *)
+Definition tbl2n_def[simp]:
+  tbl2n [] = 0n /\
+  tbl2n (T::t) = 2*tbl2n t + 1 /\
+  tbl2n (F::t) = 2*tbl2n t
+End
+
+(* binary numbers in big-endian format *)
+Overload TN2BL = “\n. REVERSE (inv_tbl2n n)”
+
+Definition inv_tbl2n_def:
+  inv_tbl2n 0n = [] /\
+  inv_tbl2n a = if EVEN a then [F]++(inv_tbl2n (a DIV 2))
+                else [T]++(inv_tbl2n ((a-1) DIV 2 ))
+Termination
+  WF_REL_TAC‘$<’ >> rw[]>>
+  irule LESS_EQ_LESS_TRANS >> qexists_tac‘v’ >> ‘0<2n’ by simp[] >>
+  rw[DIV_LE_MONOTONE,DIV_LESS,DIV_LESS_EQ]
+End
+
+Theorem tbl2n_inv_tbl2n[simp]:
+  tbl2n (inv_tbl2n n) = n
+Proof
+  completeInduct_on ‘n’ >> Cases_on‘n’ >> simp[tbl2n_def,inv_tbl2n_def] >>
+  Cases_on‘EVEN (SUC n')’ >>
+  simp[tbl2n_def]
+  >- (‘2 * (SUC n' DIV 2) = (SUC n' DIV 2)*2’ by simp[MULT_COMM] >>
+      ‘0<2n’ by simp[] >>
+      ‘SUC n' MOD 2=0’ by metis_tac[EVEN_MOD2] >>
+      ‘SUC n' DIV 2 * 2 + SUC n' MOD 2 = SUC n'’ by metis_tac[GSYM DIVISION] >>
+      fs[])
+  >- (‘0<2n’ by simp[] >> ‘n' DIV 2 <= n'’ by simp[DIV_LESS_EQ] >>
+      ‘n' DIV 2 < SUC n'’ by
+        simp[LESS_EQ_IMP_LESS_SUC] >> fs[] >>
+      ‘EVEN n'’ by metis_tac[ODD,EVEN_OR_ODD] >>
+      ‘2 * (n' DIV 2) =  (n' DIV 2)*2’ by simp[MULT_COMM] >> ‘0<2n’ by simp[] >>
+      ‘n' MOD 2=0’ by metis_tac[EVEN_MOD2] >>
+      ‘n' DIV 2 * 2 + n' MOD 2 = n'’ by metis_tac[GSYM DIVISION] >> fs[] )
+QED
+
+Definition pad0:
+  pad0 n bl = PAD_LEFT F n bl
+End
+
+
 Definition get_codes_from_len:
-  get_codes_from_len [] nc = [] ∧
-  get_codes_from_len (0::ls) nc = get_codes_from_len ls nc ∧
-  get_codes_from_len (l::ls) nc =
+  get_codes_from_len  [] n nc = [] ∧
+  get_codes_from_len (0::ls) n nc = get_codes_from_len ls (SUC n) nc ∧
+  get_codes_from_len (l::ls) n nc =
   let
     code = EL l nc;
     nc = LUPDATE (SUC code) l nc;
   in
-      code :: get_codes_from_len ls nc
+      (n, pad0 l $ TN2BL code) :: get_codes_from_len ls (SUC n) nc
 End
+
 
 EVAL “
  let
    ls = [3;3;3;3;3;2;4;4];
    bl = bl_count ls;
    nc = next_code bl;
-   codes = get_codes_from_len ls nc;
+   codes = get_codes_from_len ls 0 nc;
  in
     codes
  ”;
+
+
+Definition fixed_huff_tree:
+  fixed_huff_tree =
+   let
+     ls = (REPLICATE 144 8) ++ (REPLICATE 112 9) ++ (REPLICATE 24 7) ++ (REPLICATE 8 8);
+     bl = bl_count ls;
+     nc = next_code bl;
+     codes = get_codes_from_len ls 0 nc;
+   in
+     codes
+End
+EVAL “fixed_huff_tree”
+
 
 val _ = export_theory();
